Source/DafnyCompilers/Library.dfy
@@ -1,0 +1,76 @@
+module Lib {
+  module Seq {
+    function method Map<T, Q>(f: T ~> Q, ts: seq<T>) : seq<Q>
+      reads f.reads // FIXME: what does this mean?
+      requires forall t | t in ts :: f.requires(t)
+    {
+      if ts == [] then [] else [f(ts[0])] + Map(f, ts[1..])
+    }
+  }
+
+  module Datatypes {
+    datatype Option<T> =
+      | Some(t: T)
+      | None
+  }
+
+  module Str {
+    module Private {
+      function method digits(n: int, base: int): (digits: seq<int>)
+        requires base > 1
+        requires n >= 0
+        decreases n
+        ensures forall d | d in digits :: 0 <= d < base
+      {
+        if n == 0 then
+          []
+        else
+          assert n > 0;
+          assert base > 1;
+          assert n < base * n;
+          assert n / base < n;
+          digits(n / base, base) + [n % base]
+      }
+
+      function method string_of_digits(digits: seq<int>, chars: seq<char>) : string
+        requires forall d | d in digits :: 0 <= d < |chars|
+      {
+        if digits == [] then ""
+        else
+          assert digits[0] in digits;
+          assert forall d | d in digits[1..] :: d in digits;
+          [chars[digits[0]]] + string_of_digits(digits[1..], chars)
+      }
+    }
+
+    function method of_int_any(n: int, chars: seq<char>) : string
+      requires |chars| > 1
+    {
+      var base := |chars|;
+      if n == 0 then
+        "0"
+      else if n > 0 then
+        Private.string_of_digits(Private.digits(n, base), chars)
+      else
+        "-" + Private.string_of_digits(Private.digits(-n, base), chars)
+    }
+
+    const HEX_DIGITS := [
+      '0', '1', '2', '3', '4', '5', '6', '7', '8', '9',
+      'A', 'B', 'C', 'D', 'E', 'F']
+
+    function method of_int(n: int, base: int) : string
+      requires 2 <= base <= 16
+    {
+      of_int_any(n, HEX_DIGITS[..base])
+    }
+
+    method Test() { // FIXME {:test}?
+      expect of_int(0, 10) == "0";
+      expect of_int(3, 10) == "3";
+      expect of_int(302, 10) == "302";
+      expect of_int(-3, 10) == "-3";
+      expect of_int(-302, 10) == "-302";
+    }
+  }
+}
